src/program_proof/simplepb/apps/closed_wpcs.v
@@ -5,8 +5,9 @@ From Perennial.goose_lang Require adequacy dist_adequacy.
 From Perennial.goose_lang.ffi Require grove_ffi_adequacy.
 From Perennial.program_logic Require dist_lang.
 
+From Perennial.program_proof.bank Require Import bank_proof.
 From Perennial.program_proof.simplepb Require Import pb_init_proof pb_definitions.
-From Perennial.program_proof.simplepb Require Import kvee_proof.
+From Perennial.program_proof.simplepb Require Import kv_proof.
 From Perennial.program_proof.simplepb.simplelog Require Import proof.
 From Perennial.program_proof.grove_shared Require Import urpc_proof.
 From Perennial.goose_lang Require Import crash_borrow crash_modality.
@@ -16,15 +17,16 @@ Section closed_wpcs.
 Context `{!heapGS Σ}.
 Context `{!ekvG Σ}.
 
-Definition configHost : u64 := 10.
-Lemma wpc_kv_replica_main γsys γsrv Φc fname me :
+Definition dconfigHost : u64 := 10.
+Definition lconfigHost : u64 := 110.
+Lemma wpc_kv_replica_main γsys γsrv Φc fname me configHost :
   ((∃ data' : list u8, fname f↦data' ∗ ▷ file_crash (own_Server_ghost_f γsys γsrv) data') -∗
     Φc) -∗
   config_protocol_proof.is_pb_config_host configHost γsys -∗
   is_pb_host me γsys γsrv -∗
   is_pb_system_invs γsys -∗
   (∃ data : list u8, fname f↦data ∗ file_crash (own_Server_ghost_f γsys γsrv) data) -∗
-  WPC kv_replica_main #(LitString fname) #me @ ⊤
+  WPC kv_replica_main #(LitString fname) #me #configHost @ ⊤
   {{ _, True }}
   {{ Φc }}
 .
@@ -85,5 +87,71 @@ Proof.
   wp_pures.
   done.
 Qed.
+
+Context `{!bankG Σ}.
+Lemma wp_makeBankClerk γlk kvptsto :
+  {{{
+       is_bank "init" γlk kvptsto {[ "a1"; "a2" ]}
+  }}}
+    makeBankClerk #()
+  {{{
+        γ (b:loc), RET #b; own_bank_clerk γ b {[ "a1" ; "a2" ]}
+  }}}
+.
+Proof.
+  iIntros (?) "Hpre HΦ".
+  wp_lam.
+  wp
+Qed.
+
+Lemma wp_config_main γconf {Σ} {HKV: ekvG Σ} {HG} {HL}:
+  let hG := {| goose_globalGS := HG; goose_localGS := HL |} in
+  "HconfInit" ∷ makeConfigServer_pre γconf [U64 1; U64 2] ∗
+  "#Hhost" ∷ is_config_host configHost γconf -∗
+  WP config_main #() {{ _, True }}
+.
+Proof.
+  intros ?.
+  iNamed 1.
+  wp_call.
+  wp_apply (wp_NewSlice).
+  iIntros (?) "Hsl".
+  wp_apply wp_ref_to.
+  { done. }
+  iIntros (servers_ptr) "Hservers".
+  wp_pures.
+
+  wp_apply (wp_LoadAt with "[$Hservers]").
+  iIntros "Hservers".
+  wp_apply (wp_SliceAppend with "Hsl").
+  iIntros (?) "Hsl".
+  wp_apply (wp_StoreAt with "[$Hservers]").
+  { done. }
+  iIntros "Hservers".
+
+  wp_apply (wp_LoadAt with "[$Hservers]").
+  iIntros "Hservers".
+  wp_apply (wp_SliceAppend with "Hsl").
+  iIntros (?) "Hsl".
+  wp_apply (wp_StoreAt with "[$Hservers]").
+  { done. }
+  iIntros "Hservers".
+
+  wp_apply (wp_LoadAt with "[$Hservers]").
+  iIntros "Hservers".
+  iDestruct (own_slice_to_small with "Hsl") as "Hsl".
+  rewrite replicate_0.
+  simpl.
+  wp_apply (config_proof.wp_MakeServer with "[$HconfInit $Hsl]").
+  iIntros (?) "#Hissrv".
+  wp_apply (wp_Server__Serve with "[$]").
+  {
+    iFrame "Hissrv".
+  }
+  wp_pures.
+  done.
+Qed.
+
+End closed_wpcs.
 
 End closed_wpcs.
